\documentclass{article}

\begin{document}

\title{Question: Derivation and Equivalence of \( P_0 \) in a Liquidity Pool Bonding Curve}
\author{}
\date{}
\maketitle

Consider a liquidity pool with a real bonding curve. Show that:

\[ \frac{x_0 \cdot P_{\text{high}} - y_0}{y_0 / P_{\text{low}} - x_0} = P_0 = \frac{y_0}{x_0} = \sqrt{P_{\text{high}} \cdot P_{\text{low}}} = \frac{y_{\text{int}}}{x_{\text{int}}} \]

Where \( \text{x}_{\text{int}} \) and \( \text{y}_{\text{int}} \) represent the x and y intercepts of the bonding curve respectively.

\end{document}
